src/main/scala/fi/abo/it/actortool/boogie/BasicActorTranslator.scala
@@ -8,20 +8,20 @@ class BasicActorTranslator(
     val skipMutualExclusivenessCheck: Boolean,
     val typeCtx: Resolver.Context,
     val checkContractActions: Boolean) extends EntityTranslator[BasicActor] {
-
-  val actorVerStructBuilder = new ActorVerificationStructureBuilder(stmtTranslator,typeCtx,true)
   
   def translateEntity(actor: BasicActor): List[Boogie.Decl] = {
-    val avs = actorVerStructBuilder.buildStructure(actor)
+    val avs = VerStruct(actor, checkContractActions)
     translateActor(avs)
   }
   
-  def translateActor(avs: ActorVerificationStructure): List[Boogie.Decl] = {    
+  def translateActor(avs: ActorVerStruct): List[Boogie.Decl] = {    
     val decls = new ListBuffer[Boogie.Decl]()
     val actionFiringRules = collection.mutable.Map[AbstractAction,(Boogie.Expr,Boogie.Expr)]()
     val nonLocalActionFiringRules = collection.mutable.Map[AbstractAction,(Boogie.Expr,Boogie.Expr)]()
     val actionInpatDecls = collection.mutable.Map[AbstractAction,List[BDecl]]()
     val actionRenamings = collection.mutable.Map[AbstractAction,Map[String,Id]]()
+    val gts = collection.mutable.Map[AbstractAction,GuardTranslation]()
+    
     var allInpatDecls = Set.empty[BDecl]
     
     if (checkContractActions) {
@@ -31,29 +31,31 @@ class BasicActorTranslator(
     
     decls += translateActorInit(avs)
     
-    for (a <- avs.actorActions) {
+    for (a <- avs.entity.actorActions) {
       if (!a.init) {
-        val (patterns,guards,nonLocalGuards,inpatDecls,renamings) = translateActorGuards(a, avs)
-        allInpatDecls = allInpatDecls ++ inpatDecls
-        actionFiringRules += (a -> (patterns,guards))
-        nonLocalActionFiringRules += (a -> (patterns,nonLocalGuards))
-        actionInpatDecls += (a -> inpatDecls)
-        actionRenamings += (a -> renamings)
+        val gt = translateActorGuards(a, avs)
+        gts += (a -> gt)
+        allInpatDecls = allInpatDecls ++ gt.declarations
+        actionFiringRules += (a -> (gt.pattern,gt.localGuard))
+        nonLocalActionFiringRules += (a -> (gt.pattern,gt.localGuard))
+        actionInpatDecls += (a -> gt.declarations.toList)
+        actionRenamings += (a -> gt.renamings)
       }
     }
     
-    for (a <- avs.actorActions) {
+    for (a <- avs.entity.actorActions) {
       if (!a.init) {
-        val higherPrioActions = avs.priorityMap(a)
+        val higherPrioActions = avs.priorities(checkContractActions)(a)
         val higherPrioGuards = higherPrioActions map { h => actionFiringRules(h) }
-        decls ++= translateActorAction(a, avs, allInpatDecls.toList, avs.renamings ++ actionRenamings(a), actionFiringRules(a), higherPrioGuards)
+        val vs = VerStruct(avs,a,gts(a))
+        decls ++= translateActorAction(a, vs, higherPrioGuards)
       }
     }
     
     val allGuards = new ListBuffer[(AbstractAction,Boogie.Expr)]()
     //val supersetTests = new ListBuffer[Boogie.Expr]()
     
-    for ((action,higherPrioActions) <- avs.priorityMap) {
+    for ((action,higherPrioActions) <- avs.priorities(checkContractActions)) {
       val (ownPattern,ownGuard) = nonLocalActionFiringRules(action)
       val negHigherPrioGuards = higherPrioActions map { a => { val (p,g) = nonLocalActionFiringRules(a); Boogie.UnaryExpr("!",p && g) } }
 
@@ -72,13 +74,13 @@ class BasicActorTranslator(
     
     if (checkContractActions) {
       val contractActionFiringRules = new ListBuffer[(AbstractAction,Boogie.Expr)]
-      for (a <- avs.contractActions) {
+      for (a <- avs.contracts) {
         val firingRule = new ListBuffer[Boogie.Expr]
         for (p <- a.inputPattern) {
           firingRule += B.Int(p.rate) <= B.Urd(p.portId)
           decls += translateContractActionInput(avs, p, a)
         }
-        firingRule ++= a.guards map { p => transExpr(p)(avs.renamings) }
+        firingRule ++= a.guards map { p => transExpr(p,avs) }
         decls ++= translateContractActionExit(avs, a, allGuards.toList)
         
         contractActionFiringRules += (( a, firingRule.foldLeft(B.Bool(true): Boogie.Expr)((a,b) => a && b) ))
@@ -91,21 +93,21 @@ class BasicActorTranslator(
         }
       }
     }
+    
     decls.toList
   }
   
   def createMutualExclusivenessCheck(
-      avs: ActorVerificationStructure, guards: List[(AbstractAction,Boogie.Expr)], inpatDecls: Set[BDecl]): Option[Boogie.Proc] = {
+      avs: ActorVerStruct, guards: List[(AbstractAction,Boogie.Expr)], inpatDecls: Set[BDecl]): Option[Boogie.Proc] = {
     
-    val nonInitActions = (avs.actorActions.filter { a => !a.init }).size
+    val nonInitActions = (avs.entity.actorActions.filter { a => !a.init }).size
     
     if (nonInitActions > 1) {      
-      val decls = 
-        (avs.actorVarDecls map { _.decl }) ::: 
-        (inpatDecls map { _.decl }).toList ::: 
-        List(B.Assume(avs.uniquenessCondition)) :::
-        avs.basicAssumes :::
-        avs.invariants.map { inv => B.Assume(transExpr(inv.expr)(avs.renamings)) } 
+      val decls: List[Boogie.Stmt] = 
+        (avs.declarations map { _.decl }) ++ 
+        (inpatDecls map { _.decl }).toList ++
+        avs.assumes ++ 
+        avs.entity.actorInvariants.map { inv => B.Assume(transExpr(inv.expr,avs)) } 
       
       val stmt = decls ::: createMEAssertionsRec(avs.entity,guards)
       Some(B.createProc(Uniquifier.get(avs.namePrefix+B.Sep+"GuardWD"), stmt, smokeTest))
@@ -115,120 +117,115 @@ class BasicActorTranslator(
     }
   }
   
-  def translateActorInit(avs: ActorVerificationStructure) = {
-    val renamings = avs.renamings
+  def translateActorInit(avs1: ActorVerStruct) = {
+    //val renamings = avs.renamings
+    
+    val initAction = avs1.entity.actorActions.find( x => x.init ).get
+    
+    val vs = VerStruct(
+        avs1,
+        initAction,
+        GuardTranslation(initAction,Seq.empty,Map.empty,B.Bool(true),B.Bool(true),B.Bool(true)))
     
     val asgn = new ListBuffer[Boogie.Stmt]
-    //asgn ++= avs.channelDecls map { _.decl }
-    asgn ++= avs.actorVarDecls map { _.decl }
-    asgn ++= avs.actorParamDecls map { _.decl }
-    asgn += B.Assume(avs.uniquenessCondition)
-    asgn ++= avs.initAssumes
     
-    val initAction = avs.actorActions.find { x => x.init } 
-    initAction match {
-      case Some(a) => {
-        asgn ++= stmtTranslator.transStmt(a.body, TranslatorContext(avs.renamings,false,avs.stateChanRenamings))
-        
-        //asgn ++= transStmt( a.body )(avs.renamings)
-        for (q <- a.ensures) {
-          if (!q.free) {
-            asgn += B.Assert(transExpr(q.expr)(avs.renamings), q.pos, "Action postcondition might not hold")
-          }
-        }
-        for (opat <- a.outputPattern) {
-          val cId = opat.portId
-          for (v <- opat.exps) {
-            asgn += Boogie.Assign(B.ChannelIdx(cId, v.typ, B.C(cId)), transExpr(v)(avs.renamings))
-            asgn += Boogie.Assign(B.C(cId), B.C(cId) plus B.Int(1))
-          }
-        }
+    asgn ++= vs.declarations map { _.decl }
+    
+    asgn ++= vs.assumes
+    
+    asgn ++= stmtTranslator.transStmt(initAction.body, TranslatorContext(vs.renamings,false,vs.stateChannelNames))
+    
+    //asgn ++= transStmt( a.body )(avs.renamings)
+    for (q <- initAction.ensures) {
+      if (!q.free) {
+        asgn += B.Assert(transExpr(q.expr,vs), q.pos, "Action postcondition might not hold")
       }
-      case None =>
+    }
+    for (opat <- initAction.outputPattern) {
+      val cId = opat.portId
+      for (v <- opat.exps) {
+        asgn += Boogie.Assign(B.ChannelIdx(cId, v.typ, B.C(cId)), transExpr(v,vs))
+        asgn += Boogie.Assign(B.C(cId), B.C(cId) plus B.Int(1))
+      }
     }
     
-    for ((id,ch) <- avs.stateChanRenamings) {
-      asgn += Boogie.Assign(B.ChannelIdx(transExpr(ch)(renamings),B.C(transExpr(ch)(renamings))), transExpr(Id(id).withType(ch.typ))(renamings) )
-      asgn += Boogie.Assign(B.C(transExpr(ch)(renamings)),B.C(transExpr(ch)(renamings)) + B.Int(1))
+    for ((id,ch) <- vs.stateChannelNames) {
+      asgn += Boogie.Assign(
+          B.ChannelIdx(transExpr(ch,vs),B.C(transExpr(ch,vs))), 
+          transExpr(Id(id).withType(ch.typ),vs) )
+      asgn += Boogie.Assign(B.C(transExpr(ch,vs)),B.C(transExpr(ch,vs)) + B.Int(1))
     }
     
-    for (inv <- avs.invariants) {
+    for (inv <- vs.parent.entity.actorInvariants) {
       if (!inv.assertion.free) 
-        asgn += B.Assert(transExpr(inv.expr)(avs.renamings),inv.expr.pos, "Initialization might not establish the invariant")
+        asgn += B.Assert(transExpr(inv.expr,vs),inv.expr.pos, "Initialization might not establish the invariant")
     }
     
-    B.createProc(Uniquifier.get(avs.namePrefix+"init"),asgn.toList,smokeTest)
+    B.createProc(Uniquifier.get(vs.namePrefix+B.Sep+"init"),asgn.toList,smokeTest)
   }
   
   
   
   def translateActorAction(
       a: ActorAction, 
-      avs: ActorVerificationStructure,
-      inpatDecls: List[BDecl],
-      renamings: Map[String,Id], 
-      guard1: (Boogie.Expr,Boogie.Expr),
+      vs: ActionVerStruct,
       higherPrioGuards: List[(Boogie.Expr,Boogie.Expr)]): List[Boogie.Decl] = {
      
     val asgn = new ListBuffer[Boogie.Stmt]
-    val actionData = avs.actionData(a)
     
-    //asgn ++= avs.channelDecls map { _.decl }
-    asgn ++= avs.actorVarDecls map { _.decl }
-    asgn ++= avs.actorParamDecls map { _.decl }
-    asgn ++= inpatDecls map { _.decl }
-    asgn ++= actionData.declarations map { _.decl }
-    asgn += B.Assume(avs.uniquenessCondition)
-    
-    if (a.init) asgn ++= avs.initAssumes
-    else asgn ++= avs.basicAssumes
+    val invariants = vs.parent.entity.actorInvariants
+
+    asgn ++= vs.declarations map { _.decl }
+    //asgn ++= vs.de map { _.decl }
+    asgn ++= vs.assumes
+
+//    if (a.init) asgn ++= avs.initAssumes
+//    else asgn ++= avs.basicAssumes
      
     if (!a.init) {
       // Assume invariants
-      asgn ++= (for (i <- avs.invariants) yield B.Assume(transExpr(i.expr)(avs.renamings)))
+      asgn ++= (for (i <- invariants) yield B.Assume(transExpr(i.expr,vs.parent)))
     }
 
-    for ((id,ch) <- avs.stateChanRenamings) {
-      asgn += B.Assume(B.ChannelIdx(transExpr(ch)(renamings),B.R(transExpr(ch)(renamings))) ==@ transExpr(Id(id).withType(ch.typ))(renamings))
-      asgn += Boogie.Assign(B.R(transExpr(ch)(renamings)),B.R(transExpr(ch)(renamings)) + B.Int(1))
+    for ((id,ch) <- vs.stateChannelNames) {
+      asgn += B.Assume(B.ChannelIdx(transExpr(ch,vs),B.R(transExpr(ch,vs))) ==@ transExpr(Id(id).withType(ch.typ),vs))
+      asgn += Boogie.Assign(B.R(transExpr(ch,vs)),B.R(transExpr(ch,vs)) + B.Int(1))
     }
     
     // Assume input pattern
-    asgn ++= ( guard1 match { case (pat,_) => List(B.Assume(pat)) } )
+    asgn += B.Assume(vs.guard.pattern)
     
     for (ipat <- a.inputPattern) {
       val cId = ipat.portId
       if (ipat.repeat == 1) {
         for (v <- ipat.vars) {
-          asgn += Boogie.Assign(transExpr(v)(renamings), B.ChannelIdx(cId, v.typ, B.R(cId)))
+          asgn += Boogie.Assign(transExpr(v,vs), B.ChannelIdx(cId, v.typ, B.R(cId)))
           asgn += Boogie.Assign(B.R(cId), B.R(cId) plus B.Int(1))
         }
       }
       else {
         val v = ipat.vars(0)
         for (i <- 0 until ipat.repeat) {
-          asgn += Boogie.Assign(transExpr(v)(renamings), B.Fun("Map#Store",transExpr(v)(renamings) , B.Int(i) , B.ChannelIdx(cId, v.typ, B.R(cId)) )  )
+          asgn += Boogie.Assign(transExpr(v,vs), B.Fun("Map#Store",transExpr(v,vs) , B.Int(i) , B.ChannelIdx(cId, v.typ, B.R(cId)) )  )
           asgn += Boogie.Assign(B.R(cId), B.R(cId) plus B.Int(1))
         }
       }
     }
     
     for (p <- a.requires) {
-      asgn += B.Assume(transExpr(p.expr)(renamings))
+      asgn += B.Assume(transExpr(p.expr,vs))
     }
 
     asgn ++= higherPrioGuards map { case (pat,guard) => B.Assume(Boogie.UnaryExpr("!", /*pat &&*/ guard)) }
     
-    asgn ++= ( guard1 match { case (_,guard) => List(B.Assume(guard)) } )
-    asgn ++= actionData.variableInitialValues map { a => B.Assume(transExpr(a)(renamings) ) }
-    //asgn ++= transStmt( a.body )(renamings)
-    asgn ++= stmtTranslator.transStmt(a.body, TranslatorContext(renamings,false,avs.stateChanRenamings))
+    asgn += B.Assume(vs.guard.localGuard)
+    asgn ++= vs.actionVariableInits map { a => B.Assume(transExpr(a,vs) ) }
     
-    val transCtx = TranslatorContext(renamings,false,avs.stateChanRenamings)
+    asgn ++= transStmt(a.body, vs)
     
     for (q <- a.ensures) {
       if (!q.free) {
-        asgn += B.Assert(stmtTranslator.transExpr(q.expr, transCtx), q.pos, "Action postcondition might not hold")
+        asgn += B.Assert(transExpr(q.expr, vs), q.pos, "Action postcondition might not hold")
       }
     }
      
@@ -236,83 +233,82 @@ class BasicActorTranslator(
       val cId = opat.portId
       if (opat.repeat == 1) {
         for (v <- opat.exps) {
-          asgn += Boogie.Assign(B.ChannelIdx(cId, v.typ, B.C(cId)), transExpr(v)(renamings))
+          asgn += Boogie.Assign(B.ChannelIdx(cId, v.typ, B.C(cId)), transExpr(v,vs))
           asgn += Boogie.Assign(B.C(cId), B.C(cId) plus B.Int(1))
         }
       }
       else {
         val v = opat.exps(0)
         for (i <- 0 until opat.repeat) {
-          asgn += Boogie.Assign(B.ChannelIdx(cId, v.typ, B.C(cId)), B.Fun("Map#Select",transExpr(v)(renamings), B.Int(i)))
+          asgn += Boogie.Assign(B.ChannelIdx(cId, v.typ, B.C(cId)), B.Fun("Map#Select",transExpr(v,vs), B.Int(i)))
           asgn += Boogie.Assign(B.C(cId), B.C(cId) plus B.Int(1))
         }
       }
     }
     
-    for ((id,ch) <- avs.stateChanRenamings) {
-      asgn += Boogie.Assign(B.ChannelIdx(transExpr(ch)(renamings),B.C(transExpr(ch)(renamings))), transExpr(Id(id).withType(ch.typ))(renamings) )
-      asgn += Boogie.Assign(B.C(transExpr(ch)(renamings)),B.C(transExpr(ch)(renamings)) + B.Int(1))
+    for ((id,ch) <- vs.stateChannelNames) {
+      asgn += Boogie.Assign(B.ChannelIdx(transExpr(ch,vs),B.C(transExpr(ch,vs))), transExpr(Id(id).withType(ch.typ),vs) )
+      asgn += Boogie.Assign(B.C(transExpr(ch,vs)),B.C(transExpr(ch,vs)) + B.Int(1))
     }
      
-    for (inv <- avs.invariants) {
+    for (inv <- invariants) {
       if (!inv.assertion.free) 
-        asgn += B.Assert(transExpr(inv.expr)(avs.renamings),inv.expr.pos, "Action '" + a.fullName +  "' at " + a.pos + " might not preserve the invariant")
+        asgn += B.Assert(transExpr(inv.expr,vs.parent),inv.expr.pos, "Action '" + a.fullName +  "' at " + a.pos + " might not preserve the invariant")
     }
      
-    val proc = B.createProc(Uniquifier.get(avs.namePrefix+a.fullName),asgn.toList,smokeTest)
+    val proc = B.createProc(Uniquifier.get(vs.namePrefix),asgn.toList,smokeTest)
      
     List(proc)
   }
   
   
   
-  def generateCommonContractProcedureHeader(avs: ActorVerificationStructure, action: ContractAction) = {
+  def generateCommonContractProcedureHeader(avs: VerStruct[BasicActor], action: ContractAction) = {
     val asgn = new ListBuffer[Boogie.Stmt]
     
     //asgn ++= avs.channelDecls map { _.decl }
-    asgn ++= avs.actorVarDecls map { _.decl }
-    asgn ++= avs.actorParamDecls map { _.decl }
-    asgn += B.Assume(avs.uniquenessCondition)
-    asgn ++= avs.basicAssumes
+    asgn ++= avs.declarations.map(_.decl)
+    asgn ++= avs.assumes
     asgn += B.Assume(B.Mode(B.This) ==@ Boogie.VarExpr(action.fullName))
     
     for (op <- avs.entity.outports) {
       asgn += B.Assume(B.R(op.id) ==@ B.I(op.id))
     }
     
-    asgn ++= { for (i <- avs.invariants) yield B.Assume(transExpr(i.expr)(avs.renamings)) }
+    asgn ++= { for (i <- avs.entity.actorInvariants) yield B.Assume(transExpr(i.expr,avs)) }
     
     asgn.toList
   }
   
   
-  def translateContractActionInput(avs: ActorVerificationStructure, pattern: NwPattern,  action: ContractAction) = {
+  def translateContractActionInput(avs: VerStruct[BasicActor], pattern: NwPattern,  action: ContractAction) = {
     val asgn = new ListBuffer[Boogie.Stmt]
     asgn ++= generateCommonContractProcedureHeader(avs, action)
     
     val portType = avs.entity.getInport(pattern.portId).get.portType
-    val portVar = transExpr(pattern.portId,ChanType(portType))(avs.renamings)
+    val portVar = transExpr(pattern.portId,ChanType(portType),avs)
     asgn += B.Assume(B.C(portVar) - B.I(portVar) < B.Int(pattern.rate))
     
     asgn += Boogie.Assign(B.C(portVar), B.C(portVar) + B.Int(1))
         
     for (r <- action.requires) {
-      asgn += B.Assume(transExpr(r.expr)(avs.renamings))
-    }
-    for (r <- action.guards) {
-      asgn += B.Assume(transExpr(r)(avs.renamings))
+      asgn += B.Assume(transExpr(r.expr,avs))
     }
     
-    for (chi <- avs.invariants) {
+    for (r <- action.guards) {
+      asgn += B.Assume(transExpr(r,avs))
+    }
+    
+    for (chi <- avs.entity.actorInvariants) {
       if (!chi.assertion.free) {
-        asgn += BAssert(chi, "Invariant might be falsified by actor input", avs.renamings)
+        asgn += BAssert(chi, "Invariant might be falsified by actor input", avs)
       }
     }
     B.createProc(Uniquifier.get(avs.namePrefix+"contract"+B.Sep+action.fullName+B.Sep+"input"), asgn.toList, smokeTest)
   }
   
   
-  def translateContractActionExit(avs: ActorVerificationStructure, action: ContractAction, guards: List[(AbstractAction, Boogie.Expr)]) = {
+  def translateContractActionExit(avs: VerStruct[BasicActor], action: ContractAction, guards: List[(AbstractAction, Boogie.Expr)]) = {
     val asgn = new ListBuffer[Boogie.Stmt]
     asgn ++= generateCommonContractProcedureHeader(avs, action)
     
@@ -322,7 +318,7 @@ class BasicActorTranslator(
     }
       
     for (p <- action.requires) {
-      asgn += B.Assume(transExpr(p.expr)(avs.renamings))
+      asgn += B.Assume(transExpr(p.expr,avs))
     }
     
     for ((_,g) <- guards) {
@@ -337,7 +333,7 @@ class BasicActorTranslator(
     
     for (q <- action.ensures) {
       if (!q.free) {
-        asgn += B.Assert(transExpr(q.expr)(avs.renamings),q.pos,"Contract action postcondition might not hold")
+        asgn += B.Assert(transExpr(q.expr,avs),q.pos,"Contract action postcondition might not hold")
       }
     }
     
@@ -346,9 +342,9 @@ class BasicActorTranslator(
     }
     asgn += Boogie.Assign(Boogie.VarExpr(BMap.I), Boogie.VarExpr(BMap.R))
     
-    for (inv <- avs.invariants) {
+    for (inv <- avs.entity.actorInvariants) {
       if (!inv.assertion.free) {
-        asgn += BAssert(inv,"The actor might not preserve the invariant with contract '" + action.fullName + "' at " + action.pos, avs.renamings)
+        asgn += BAssert(inv,"The actor might not preserve the invariant with contract '" + action.fullName + "' at " + action.pos,avs)
       }
     }
     
