src/main/scala/fi/abo/it/actortool/boogie/BoogieScheduleCheckTranslator.scala
@@ -3,7 +3,11 @@ package fi.abo.it.actortool.boogie
 import fi.abo.it.actortool._
 import fi.abo.it.actortool.schedule._
 
-class BoogieScheduleCheckTranslator(mergedActions: Boolean, actionTranslator: BasicActorTranslator) extends EntityTranslator[ScheduleContext] with GeneralBackend[ScheduleContext,List[Boogie.Decl]] {
+class BoogieScheduleCheckTranslator(
+    mergedActions: Boolean, 
+    actionTranslator: BasicActorTranslator) 
+    extends EntityTranslator[ScheduleContext] 
+    with GeneralBackend[ScheduleContext,List[Boogie.Decl]] {
 
   
   def invoke(scheduleCtx: ScheduleContext) = translateEntity(scheduleCtx)
@@ -20,93 +24,86 @@ class BoogieScheduleCheckTranslator(mergedActions: Boolean, actionTranslator: Ba
         }
       }).flatten
     
-    val decls = scheduleCtx.entity match {
-      case nw: Network => {
-        val verStructBuilder = new NetworkVerificationStructureBuilder(stmtTranslator,new Resolver.EmptyContext(true),mergedActions)
-        val nwvs = verStructBuilder.buildStructure(nw)
-        scheduleCtx.schedules.flatMap(s => translateNetworkSchedule(scheduleCtx, s, nwvs))
-      }
-      case ba: BasicActor => {
-        val verStructBuilder = new ActorVerificationStructureBuilder(stmtTranslator,new Resolver.EmptyContext(true),mergedActions)
-        val avs = verStructBuilder.buildStructure(ba)
-        
-        val actionChecks = actionTranslator.translateActor(avs)
-        
-        translateFunctionDecl(avs) ::: actionChecks ::: scheduleCtx.schedules.flatMap(s => translateActorSchedule(scheduleCtx,s,avs))
+      
+    val decls = {
+      scheduleCtx.entity match {
+        case ba: BasicActor => {
+          val vs = VerStruct(ba,mergedActions)
+            
+          translateFunctionDecl(vs) ++ 
+          //actionChecks ++ 
+          scheduleCtx.schedules.flatMap { s => translateActorSchedule(scheduleCtx,s,vs) }
+        }
+        case nw: Network => {
+          val vs = VerStruct(nw,mergedActions)
+          scheduleCtx.schedules.flatMap {
+            s => translateNetworkSchedule(scheduleCtx, s, vs)
+          }
+        }
       }
     }
-      
-    constDecls ::: decls
+    
+    constDecls ++ decls
   }
   
-  def translateActorSchedule(scheduleCtx: ScheduleContext, schedule: ContractSchedule, avs: ActorVerificationStructure) = {
+  def translateActorSchedule(scheduleCtx: ScheduleContext, schedule: ContractSchedule, avs: RootVerStruct[BasicActor]) = {
     val decls = new collection.mutable.ListBuffer[Boogie.Stmt]
     val stmts = new collection.mutable.ListBuffer[Boogie.Stmt]
     val alreadyDeclared = collection.mutable.Set[String]()
-    decls ++= avs.actorVarDecls map { _.decl }
-    decls ++= avs.actorParamDecls map { _.decl }
-    stmts += B.Assume(avs.uniquenessCondition)
-    stmts ++= avs.basicAssumes
+    
+    decls ++= avs.declarations.map(_.decl)
+    alreadyDeclared ++= avs.declarations.map(_.name)
+    stmts ++= avs.assumes
+    
     stmts += B.Assume(B.Mode(B.This) ==@ Boogie.VarExpr(schedule.contract.fullName))
     stmts += B.Assume(Boogie.VarExpr(BMap.R) ==@ Boogie.VarExpr(BMap.I))
     stmts += B.Assume(Boogie.VarExpr(BMap.C) ==@ Boogie.VarExpr(BMap.R))
-    for (inv <- avs.invariants) stmts += BAssume(inv, avs.renamings)
+    
+    for (inv <- avs.entity.actorInvariants) stmts += BAssume(inv, avs)
     
     for (ipat <- schedule.contract.inputPattern) {
       stmts += Boogie.Assign(
-          B.C(transExpr(ipat.portId,ipat.typ)(avs.renamings)), 
-          B.C(transExpr(ipat.portId,ipat.typ)(avs.renamings)) + B.Int(ipat.rate))
+          B.C(transExpr(ipat.portId,ipat.typ,avs)), 
+          B.C(transExpr(ipat.portId,ipat.typ,avs)) + B.Int(ipat.rate))
     }
     
-    stmts ++= schedule.contract.guards.map { g => B.Assume(transExpr(g)(avs.renamings)) }
-    stmts ++= schedule.contract.requires.map { r => B.Assume(transExpr(r.expr)(avs.renamings)) }
+    stmts ++= schedule.contract.guards.map { g => B.Assume(transExpr(g,avs)) }
+    stmts ++= schedule.contract.requires.map { r => B.Assume(transExpr(r.expr,avs)) }
     
-    val renamingsBuffer = collection.mutable.Map[ActorAction,Map[String,Id]]()
-    for (action <- schedule.entity.actorActions) {
-      val prefix = action.fullName
-      val actionRenamings = collection.mutable.Map[String,Id]()
-      for (v <- action.variables) {
-        val name = prefix+B.Sep+v.id
-        decls += B.Local(name,B.type2BType(v.typ))
-        val id = Id(name)
-        id.typ = v.typ
-        actionRenamings += (v.id -> id)
-      }
-      for (p <- action.inputPattern) {
-        for (v <- p.vars) {
-          val name = prefix+B.Sep+v.id
-          decls += B.Local(name,B.type2BType(v.typ))
-          val id = Id(name)
-          id.typ = v.typ
-          actionRenamings += (v.id -> id)
-        }
-      }
-      renamingsBuffer += (action -> actionRenamings.toMap)
-    }
-    
-    val renamings = renamingsBuffer.toMap
     
     for (firing <- schedule.sequence) {
       val action = firing.action
-      val actionRenamings = avs.renamings ++ renamings(action)
-      val actionData = avs.actionData(action)
+
+      val gt = translateActorGuards(action, avs)
+      
+      val tvs = VerStruct(avs,action,gt,true)
+      
+      for (d <- tvs.declarations) {
+        if (!alreadyDeclared.contains(d.name)) {
+          decls += d.decl
+          alreadyDeclared += d.name
+        }
+      }
       
       for (ipat <- action.inputPattern) {
         val id = ipat.portId
-        stmts += B.Assert(B.Int(ipat.rate) <= B.Urd(id),ipat.pos,"Input pattern might not be satisfied for action '" + action.fullName + "'")
+        stmts += B.Assert(
+            B.Int(ipat.rate) <= B.Urd(id),
+            ipat.pos,
+            "Input pattern might not be satisfied for action '" + action.fullName + "'")
         
         ipat match {
           case InputPattern(_,vars,1) => {
             for (v <- vars) {
-              stmts += Boogie.Assign(transExpr(v.id,v.typ)(actionRenamings),B.ChannelIdx(id,v.typ,B.R(id)))
+              stmts += Boogie.Assign(transExpr(v.id,v.typ,tvs),B.ChannelIdx(id,v.typ,B.R(id)))
               stmts += Boogie.Assign(B.R(id), B.R(id) + B.Int(1))
             }
           }
           case InputPattern(_,List(v),repeat) => {
             for (i <- 0 until repeat) {
               stmts += Boogie.Assign(
-                  transExpr(v)(actionRenamings), 
-                  B.Fun("Map#Store",transExpr(v)(actionRenamings) , B.Int(i) , B.ChannelIdx(id, v.typ, B.R(id)) )  )
+                  transExpr(v,tvs), 
+                  B.Fun("Map#Store",transExpr(v,tvs) , B.Int(i) , B.ChannelIdx(id, v.typ, B.R(id)) )  )
               stmts += Boogie.Assign(B.R(id), B.R(id) plus B.Int(1))
             }
           }
@@ -114,12 +111,22 @@ class BoogieScheduleCheckTranslator(mergedActions: Boolean, actionTranslator: Ba
         }
         
       }
-      stmts ++= action.guards.map { g => B.Assert(transExpr(g)(actionRenamings),g.pos,"Guard might not be satisfied for action '" + action.fullName + "'" ) }
-      stmts ++= action.requires.filter(!_.free).map { r => B.Assert(transExpr(r.expr)(actionRenamings),r.pos,"Precondition might not hold for action '" + action.fullName + "'" ) }
       
-      stmts ++= generateHavoc(actionData.assignedVariables, actionRenamings)
+      stmts ++= action.guards.map { 
+        g => B.Assert(
+            transExpr(g,tvs),
+            g.pos,
+            "Guard might not be satisfied for action '" + action.fullName + "'" ) 
+      }
       
-      //stmts ++= transStmt(action.body)(actionRenamings)
+      stmts ++= action.requires.filter(!_.free).map { 
+        r => B.Assert(
+            transExpr(r.expr,tvs),
+            r.pos,
+            "Precondition might not hold for action '" + action.fullName + "'" ) 
+      }
+      
+      stmts ++= generateHavoc(tvs.assignedVariables,tvs)
       
       for (opat <- action.outputPattern) {
         val id = opat.portId
@@ -127,26 +134,26 @@ class BoogieScheduleCheckTranslator(mergedActions: Boolean, actionTranslator: Ba
         opat match {
           case OutputPattern(_,exps,1) => {
             for (e <- exps) {
-              stmts += Boogie.Assign(B.ChannelIdx(id,e.typ,B.C(id)),transExpr(e)(actionRenamings))
+              stmts += Boogie.Assign(B.ChannelIdx(id,e.typ,B.C(id)),transExpr(e,tvs))
               stmts += Boogie.Assign(B.C(id), B.C(id) + B.Int(1))
             }
           }
           case OutputPattern(_,List(e),repeat) => {
             for (i <- 0 until repeat) {
-              stmts += Boogie.Assign(B.ChannelIdx(id, e.typ, B.C(id)), B.Fun("Map#Select",transExpr(e)(actionRenamings), B.Int(i)))
+              stmts += Boogie.Assign(B.ChannelIdx(id, e.typ, B.C(id)), B.Fun("Map#Select",transExpr(e,tvs), B.Int(i)))
               stmts += Boogie.Assign(B.C(id), B.C(id) plus B.Int(1))
             }
           }
         }
 
       }
-      for (q <- action.ensures) stmts += B.Assume(transExpr(q.expr)(actionRenamings))
-      for (inv <- avs.invariants) stmts += BAssume(inv, avs.renamings)
+      for (q <- action.ensures) stmts += B.Assume(transExpr(q.expr,tvs))
+      for (inv <- avs.entity.actorInvariants) stmts += BAssume(inv,avs)
     }
     
     for (opat <- schedule.contract.outputPattern) {
       stmts += B.Assert(
-          B.Urd(transExpr(opat.portId,opat.typ)(avs.renamings)) ==@ B.Int(opat.rate),
+          B.Urd(transExpr(opat.portId,opat.typ,avs)) ==@ B.Int(opat.rate),
           opat.pos,
           "The correct amount of tokens might not be produced on output " + opat.portId)
     }
@@ -154,52 +161,54 @@ class BoogieScheduleCheckTranslator(mergedActions: Boolean, actionTranslator: Ba
     List(B.createProc(schedule.entity.id+B.Sep+schedule.contract.fullName, decls.toList:::stmts.toList, false))
   }
   
-  def translateNetworkSchedule(scheduleCtx: ScheduleContext, schedule: ContractSchedule, nwvs: NetworkVerificationStructure) = {
+  def translateNetworkSchedule(
+      scheduleCtx: ScheduleContext, 
+      schedule: ContractSchedule, 
+      nwvs: RootVerStruct[Network]) = {
+    
     val decls = new collection.mutable.ListBuffer[Boogie.Stmt]
     val stmts = new collection.mutable.ListBuffer[Boogie.Stmt]
     val alreadyDeclared = collection.mutable.Set[String]()
     
-    decls ++= (nwvs.entityDecls map { _.decl })
-    decls ++= nwvs.subactorVarDecls map { _.decl }
+    decls ++= nwvs.declarations.map(_.decl)
+    alreadyDeclared ++= nwvs.declarations.map(_.name)
     
-    stmts ++= nwvs.uniquenessConditions map { B.Assume(_) }
-    stmts ++= nwvs.basicAssumes
+    stmts ++= nwvs.assumes
+    
     stmts += B.Assume(B.Mode(B.This) ==@ Boogie.VarExpr(schedule.contract.fullName))
     stmts += B.Assume(Boogie.VarExpr(BMap.R) ==@ Boogie.VarExpr(BMap.I))
-    for (nwi <- nwvs.nwInvariants) stmts += BAssume(nwi, nwvs.renamings)
-    for (chi <- nwvs.chInvariants) stmts += BAssume(chi, nwvs.renamings)
+    for (nwi <- nwvs.nwInvariants) stmts += BAssume(nwi, nwvs)
+    for (chi <- nwvs.chInvariants) stmts += BAssume(chi, nwvs)
     
-    for (e <- scheduleCtx.entities) {
-      val renamings = nwvs.instanceRenamings(e)
-      for (inv <- e.actor.streamInvariants) stmts += B.Assume(transExpr(inv.expr)(renamings))
-    }
+    for (ioi <- nwvs.translatedIoInvariants(stmtTranslator)) stmts += B.Assume(ioi)
     
     for (ipat <- schedule.contract.inputPattern) {
       stmts += Boogie.Assign(
-          B.C(transExpr(ipat.portId,ipat.typ)(nwvs.renamings)), 
-          B.C(transExpr(ipat.portId,ipat.typ)(nwvs.renamings)) + B.Int(ipat.rate))
+          B.C(transExpr(ipat.portId,ipat.typ,nwvs)), 
+          B.C(transExpr(ipat.portId,ipat.typ,nwvs)) + B.Int(ipat.rate))
     }
     for (guard <- schedule.contract.guards) {
-      stmts += B.Assume(transExpr(guard)(nwvs.renamings))
+      stmts += B.Assume(transExpr(guard,nwvs))
     }
     for (pre <- schedule.contract.requires) {
-      stmts += B.Assume(transExpr(pre.expr)(nwvs.renamings))
+      stmts += B.Assume(transExpr(pre.expr,nwvs))
     }
     
     for (firing <- schedule.sequence) {
       val a1 = firing.action
       val e = firing.instance
       val action = a1.refinedContract.getOrElse(a1)
-      //decls+ ++= nwvs.getEntityActionData(e, action).declarations  map { _.decl }
       
-      stmts += Boogie.Comment("Instance: " + e.id + ", Action: " + action.fullName)
-      val renamings = nwvs.subActionRenamings(e, action)
-      for (d <- nwvs.getEntityActionData(e, action).declarations) {
+      val acvs = VerStruct(VerStruct(nwvs, e), action)
+      
+      for (d <- acvs.declarations) {
         if (!alreadyDeclared.contains(d.name)) {
           decls += d.decl
           alreadyDeclared += d.name
         }
       }
+      
+      stmts += Boogie.Comment("Instance: " + e.id + ", Action: " + action.fullName)
       
       for (ip <- e.actor.inports) {
         val cId = nwvs.connectionMap.getDst(PortRef(Some(e.id),ip.id))
@@ -211,8 +220,8 @@ class BoogieScheduleCheckTranslator(mergedActions: Boolean, actionTranslator: Ba
         stmts += Boogie.Assign(B.Isub(cId), B.C(cId))
       }
       
-      val firingRules = getFiringRules(e, nwvs)
-      //println(firingRules.keys map (_.fullName))
+      val firingRules = getFiringRules(e, acvs)
+      
       stmts += B.Assert(
           firingRules(action),
           action.pos,
@@ -223,13 +232,13 @@ class BoogieScheduleCheckTranslator(mergedActions: Boolean, actionTranslator: Ba
         pat match {
           case InputPattern(_,vars,1) => {
             for (v <- vars) {
-              stmts += Boogie.Assign(transExpr(v.id,v.typ)(renamings),B.ChannelIdx(id,v.typ,B.R(id)))
+              stmts += Boogie.Assign(transExpr(v.id,v.typ,acvs),B.ChannelIdx(id,v.typ,B.R(id)))
               stmts += Boogie.Assign(B.R(id), B.R(id) plus B.Int(1))
             }
           }
           case InputPattern(_,List(v),repeat) => {
             for (i <- 0 until repeat) {
-              stmts += Boogie.Assign(transExpr(v)(renamings), B.Fun("Map#Store",transExpr(v)(renamings) , B.Int(i) , B.ChannelIdx(id, v.typ, B.R(id)) )  )
+              stmts += Boogie.Assign(transExpr(v,acvs), B.Fun("Map#Store",transExpr(v,acvs) , B.Int(i) , B.ChannelIdx(id, v.typ, B.R(id)) )  )
               stmts += Boogie.Assign(B.R(id), B.R(id) plus B.Int(1))
             }
           }
@@ -242,24 +251,24 @@ class BoogieScheduleCheckTranslator(mergedActions: Boolean, actionTranslator: Ba
       
       for (pre <- action.requires) {
         if (!pre.free) {
-          stmts += B.Assert(transExprPrecondCheck(pre.expr)(renamings),pre.pos,"Precondition might not hold")
+          stmts += B.Assert(transExprPrecondCheck(pre.expr,acvs),pre.pos,"Precondition might not hold")
         }
       }
       
-      stmts ++= generateHavoc(nwvs.getEntityActionData(e, action).assignedVariables, renamings)
+      stmts ++= generateHavoc(acvs.assignedVariables, acvs)
       
       for (pat <- action.outputPattern) {
         val id = nwvs.connectionMap.getSrc(PortRef(Some(e.id),pat.portId))
         pat match {
           case OutputPattern(_,exps,1) => {
             for (e <- exps) {
-              stmts += Boogie.Assign(B.ChannelIdx(id,e.typ,B.C(id)),transExpr(e)(renamings))
+              stmts += Boogie.Assign(B.ChannelIdx(id,e.typ,B.C(id)),transExpr(e,acvs))
               stmts += Boogie.Assign(B.C(id),B.C(id) plus B.Int(1))
             }
           }
           case OutputPattern(_,List(e),repeat) => {
             for (i <- 0 until repeat) {
-              stmts += Boogie.Assign(B.ChannelIdx(id, e.typ, B.C(id)), B.Fun("Map#Select",transExpr(e)(renamings), B.Int(i)))
+              stmts += Boogie.Assign(B.ChannelIdx(id, e.typ, B.C(id)), B.Fun("Map#Select",transExpr(e,acvs), B.Int(i)))
               stmts += Boogie.Assign(B.C(id), B.C(id) plus B.Int(1))
             }
           }
@@ -272,16 +281,16 @@ class BoogieScheduleCheckTranslator(mergedActions: Boolean, actionTranslator: Ba
       }
       
       for (post <- action.ensures) {
-        stmts += B.Assume(transExprPrecondCheck(post.expr)(renamings))
+        stmts += B.Assume(transExprPrecondCheck(post.expr,acvs))
       }
       
-      for (inv <- e.actor.streamInvariants) stmts += B.Assume(transExpr(inv.expr)(renamings))
+      for (inv <- e.actor.streamInvariants) stmts += B.Assume(transExpr(inv.expr,acvs))
       
     }
     
     for (opat <- schedule.contract.outputPattern) {
       stmts += B.Assert(
-          B.Urd(transExpr(opat.portId,opat.typ)(nwvs.renamings)) ==@ B.Int(opat.rate),
+          B.Urd(transExpr(opat.portId,opat.typ,nwvs)) ==@ B.Int(opat.rate),
           opat.pos,
           "The correct amount of tokens might not be produced on output " + opat.portId)
     }
@@ -289,11 +298,11 @@ class BoogieScheduleCheckTranslator(mergedActions: Boolean, actionTranslator: Ba
     List(B.createProc(nwvs.entity.id+B.Sep+schedule.contract.fullName, decls.toList:::stmts.toList, false))
   }
   
-  def getFiringRules(instance: Instance, nwvs: NetworkVerificationStructure) = {
+  def getFiringRules(instance: Instance, ivs: SubActionVerStruct) = {
     ///val actor = nwvs.mergedActors(instance.actorId)
     // This list includes contract actions if the entity has such, otherwise basic actions
-    val priorityList = nwvs.entityData(instance).priorities
-    (priorityList.keys map { ca => (ca, transSubActionFiringRules(instance, ca, nwvs)) }).toMap
+    val priorityList = ivs.priorities(mergedActions)
+    (priorityList.keys map { ca => (ca, transSubActionFiringRules(instance, ca, ivs)) }).toMap
   }
   
 }
