src/main/scala/fi/abo/it/actortool/boogie/NetworkTranslator.scala
@@ -7,34 +7,34 @@ import fi.abo.it.actortool.ActorTool.TranslationException
 class NetworkTranslator(
     val smokeTest: Boolean,
     val skipMutualExclusivenessCheck: Boolean,
-    val typeCtx: Resolver.Context) extends EntityTranslator[Network] {
-  
-  val nwVerStructBuilder = new NetworkVerificationStructureBuilder(stmtTranslator,typeCtx,true)
+    val typeCtx: Resolver.Context,
+    val useContracts: Boolean) extends EntityTranslator[Network] {
+
   
   def translateEntity(network: Network): List[Boogie.Decl] = {
-    val nwvs = nwVerStructBuilder.buildStructure(network)
+    val nwvs = VerStruct(network,false)
     translateNetwork(nwvs)
   }
   
-  def translateNetwork(nwvs: NetworkVerificationStructure): List[Boogie.Decl] = {
+  def translateNetwork(nwvs: RootVerStruct[Network]): List[Boogie.Decl] = {
     val decls = new ListBuffer[Boogie.Decl]()
 
     decls ++= translateNetworkInit(nwvs)
     
     val (subActorProcs, subActorFiringRules) = translateSubActorExecutions(nwvs)
     decls ++= subActorProcs
-    for (a <- nwvs.contractActions) {
-      decls ++= translateNetworkAction(a,nwvs,subActorFiringRules)
-    }
-
     
+    for (c <- nwvs.contracts) {
+      decls ++= translateNetworkAction(c,nwvs,subActorFiringRules)
+    }
+  
     val contractActionFiringRules = new ListBuffer[(AbstractAction,Boogie.Expr)]
-    for (a <- nwvs.contractActions) {
+    for (a <- nwvs.contracts) {
       val firingRule = new ListBuffer[Boogie.Expr]
       for (p <- a.inputPattern) {
-        firingRule += B.Int(p.rate) <= B.Urd(transExpr(nwvs.renamings(p.portId))(nwvs.renamings))
+        firingRule += B.Int(p.rate) <= B.Urd(transExpr(nwvs.renamings(p.portId),nwvs))
       }
-      firingRule ++= a.guards map { p => transExpr(p)(nwvs.renamings) }
+      firingRule ++= a.guards map { p => transExpr(p,nwvs) }
       
       contractActionFiringRules += (( a, firingRule.foldLeft(B.Bool(true): Boogie.Expr)((a,b) => a && b) ))
     }
@@ -50,46 +50,46 @@ class NetworkTranslator(
   }
   
   def createMutualExclusivenessCheck(
-      nwvs: NetworkVerificationStructure, guards: List[(AbstractAction,Boogie.Expr)], inpatDecls: Set[BDecl]): Option[Boogie.Proc] = {
+      nwvs: RootVerStruct[Network], guards: List[(AbstractAction,Boogie.Expr)], inpatDecls: Set[BDecl]): Option[Boogie.Proc] = {
     
     if (guards.size <= 1) return None
     
     val asgn = new ListBuffer[Boogie.Stmt]
     
-    asgn ++= (nwvs.entityDecls map { _.decl })
-    asgn ++= nwvs.subactorVarDecls map { _.decl }
-    asgn ++= nwvs.uniquenessConditions map {B.Assume(_)}
-    asgn ++= nwvs.basicAssumes
+    asgn ++= nwvs.declarations map { _.decl }
+    asgn ++= nwvs.assumes
       
     asgn ++= createMEAssertionsRec(nwvs.entity,guards)
     return Some(B.createProc(Uniquifier.get(nwvs.namePrefix+B.Sep+"GuardWD"), asgn.toList, smokeTest))
     
   }
   
-  def translateNetworkInit(nwvs: NetworkVerificationStructure): List[Boogie.Decl] = {
+  def translateNetworkInit(nwvs: RootVerStruct[Network]): List[Boogie.Decl] = {
     
     val asgn = new ListBuffer[Boogie.Stmt]
+    val connections = nwvs.entity.structure.get.connections
+    val entities = nwvs.entity.entities.get.entities
+//    asgn ++= (nwvs.entityDecls map { _.decl })
+//    asgn ++= nwvs.subactorVarDecls map { _.decl }
+//    asgn ++= nwvs.uniquenessConditions map {B.Assume(_)}
+//    asgn ++= nwvs.basicAssumes
+    asgn ++= nwvs.declarations map { _.decl }
+    asgn ++= nwvs.assumes
     
-    asgn ++= (nwvs.entityDecls map { _.decl })
-    asgn ++= nwvs.subactorVarDecls map { _.decl }
-    asgn ++= nwvs.uniquenessConditions map {B.Assume(_)}
-    asgn ++= nwvs.basicAssumes
-    
-    for (c <- nwvs.connections) {
-      asgn += B.Assume(B.C(transExpr(c.id,c.typ)(nwvs.renamings)) ==@ B.Int(0))
-      asgn += B.Assume(B.R(transExpr(c.id,c.typ)(nwvs.renamings)) ==@ B.Int(0))
+    for (c <- connections) {
+      asgn += B.Assume(B.C(transExpr(c.id,c.typ,nwvs)) ==@ B.Int(0))
+      asgn += B.Assume(B.R(transExpr(c.id,c.typ,nwvs)) ==@ B.Int(0))
     }
     
-    for (inst <- nwvs.entities) {
+    for (inst <- entities) {
+      val ivs = VerStruct(nwvs, inst)
       
       val actor = inst.actor
-      
-      val renamings = nwvs.instanceRenamings(inst)
       
       val parameterNames = actor.parameters map {x => val id = Id(x.id); id.typ = x.typ; id}
       for ((name,value) <- (parameterNames zip inst.arguments)) {
         // Add assumptions about the values of the actor parameters
-        asgn += B.Assume(transExpr(name)(renamings) ==@ transExpr(value)(renamings))
+        asgn += B.Assume(transExpr(name,ivs) ==@ transExpr(value,ivs))
       }
       
       val actions = if (actor.contractActions.isEmpty) actor.actorActions else actor.contractActions
@@ -98,7 +98,7 @@ class NetworkTranslator(
         for (opat <- ca.outputPattern) {
           val cId = nwvs.connectionMap.getSrc(inst.id,opat.portId)
           for (e <- opat.asInstanceOf[OutputPattern].exps) {
-            asgn += Boogie.Assign(B.ChannelIdx(cId,e.typ,B.C(cId)),transExpr(e)(renamings))
+            asgn += Boogie.Assign(B.ChannelIdx(cId,e.typ,B.C(cId)),transExpr(e,ivs))
             asgn += Boogie.Assign(B.C(cId),B.C(cId) plus B.Int(1))
           }
         }
@@ -108,31 +108,37 @@ class NetworkTranslator(
     
     for (chi <- nwvs.chInvariants) {
       if (!chi.assertion.free)
-        asgn += BAssert(chi, "Initialization of network '" + nwvs.entity.id + "' might not establish the channel invariant", nwvs.renamings)
+        asgn += BAssert(chi, "Initialization of network '" + nwvs.entity.id + "' might not establish the channel invariant", nwvs)
     }
     
     asgn += Boogie.Assign(Boogie.VarExpr(BMap.I), Boogie.VarExpr(BMap.R))
     for (nwi <- nwvs.nwInvariants) {
-      if (!nwi.assertion.free) 
-        asgn += BAssert(nwi,"Initialization of network '" + nwvs.entity.id + "' might not establish the network invariant",nwvs.renamings)
+      if (!nwi.assertion.free) {
+        asgn += BAssert(nwi,"Initialization of network '" + nwvs.entity.id + "' might not establish the network invariant",nwvs)
+      }
     }
     
     val stmt = asgn.toList
     List(B.createProc(Uniquifier.get(nwvs.namePrefix+"init"),stmt,smokeTest))
   }
   
-  def translateSubActorExecutions(nwvs: NetworkVerificationStructure) = {
+  def translateSubActorExecutions(nwvs: RootVerStruct[Network]) = {
     
     val boogieProcs = new ListBuffer[Boogie.Proc]()
     val nwFiringRules = new ListBuffer[Boogie.Expr]()
     
     for (inst <- nwvs.entities) {
+      val ivs = VerStruct(nwvs, inst)
       val actor = inst.actor
       
       /// This list includes contract actions if the entity has such, otherwise basic actions
-      val priorityList = nwvs.entityData(inst).priorities
+      val priorityList = ivs.priorities(useContracts)
       
-      val firingRules = (priorityList.keys map { ca => (ca, transSubActionFiringRules(inst, ca, nwvs)) }).toMap
+      val firingRules = (priorityList.keys map { 
+        ca => 
+          val acvs = VerStruct(ivs, ca)
+          (ca, transSubActionFiringRules(inst, ca, acvs)) 
+      }).toMap
       
       for ((ca,higherPrioActions) <- priorityList) {
         if (!ca.init) {
@@ -140,7 +146,8 @@ class NetworkTranslator(
           
           val higherPrioFiringRules = higherPrioActions map {a => firingRules(a) }
           
-          val subActorStmt = transSubActionExecution(inst, ca, nwvs, firingRules(ca))
+          val acvs = VerStruct(ivs, ca)
+          val subActorStmt = transSubActionExecution(inst, ca, acvs, firingRules(ca))
           boogieProcs += B.createProc(Uniquifier.get(procName),subActorStmt,smokeTest)
         }
       }
@@ -150,9 +157,126 @@ class NetworkTranslator(
     (boogieProcs.toList, nwFiringRules.toList)
   }
   
-  def translateNetworkAction(
-      nwa: ContractAction, nwvs: NetworkVerificationStructure, subactorFiringRules: List[Boogie.Expr]): List[Boogie.Decl] = {
+  def transSubActionExecution(
+      instance: Instance, 
+      action: AbstractAction, 
+      acvs: SubActionVerStruct,
+      firingRule: Boogie.Expr): List[Boogie.Stmt] = {
     
+    val actor = instance.actor
+    
+    val asgn = new ListBuffer[Boogie.Stmt]()
+    
+//    asgn ++= nwvs.entityDecls map { _.decl }
+//    asgn ++= nwvs.subactorVarDecls  map { _.decl }
+//    asgn ++= nwvs.uniquenessConditions map {B.Assume(_)}
+//    asgn ++= nwvs.getEntityActionData(instance, action).declarations  map { _.decl }
+//    
+//    asgn ++= nwvs.basicAssumes
+//    
+    asgn ++= acvs.declarations.map { _.decl }
+    asgn ++= acvs.assumes
+    
+    
+    for (ip <- instance.actor.inports) {
+      val cId = acvs.connectionMap.getDst(PortRef(Some(instance.id),ip.id))
+      asgn += Boogie.Assign(B.Isub(cId), B.R(cId))
+    }
+    
+    for (op <- instance.actor.outports) {
+      val cId = acvs.connectionMap.getSrc(PortRef(Some(instance.id),op.id))
+      asgn += Boogie.Assign(B.Isub(cId), B.C(cId))
+    }
+    
+    asgn ++= (for (chi <- acvs.chInvariants) yield BAssume(chi,acvs))  // Assume channel invariants
+    
+    asgn ++= acvs.parent.parent.translatedIoInvariants(stmtTranslator) map B.Assume
+    
+//    for ((pinv,renames) <- nwvs.publicSubInvariants) {
+//      asgn += BAssume(pinv, renames)
+//    }
+    
+//    val renamings = nwvs.subActionRenamings(instance, action)
+//    
+//    val replacementMap = nwvs.getEntityActionData(instance, action).replacements
+//    
+    asgn += B.Assume(firingRule)
+    
+    for (ipat <- action.inputPattern) {
+      val cId = acvs.connectionMap.getDst(PortRef(Some(instance.id),ipat.portId))
+      if (action.isContractAction) {
+        asgn += Boogie.Assign(B.R(cId), B.R(cId) plus B.Int(ipat.rate))
+      }
+      else {
+        val inputPat = ipat.asInstanceOf[InputPattern]
+        if (inputPat.repeat == 1) {
+          for (v <- inputPat.vars) {
+            asgn += Boogie.Assign(transExpr(v.id,v.typ,acvs),B.ChannelIdx(cId,v.typ,B.R(cId)))
+            asgn += Boogie.Assign(B.R(cId), B.R(cId) plus B.Int(1))
+          }
+        }
+        else {
+          val v = inputPat.vars(0)
+          for (i <- 0 until inputPat.repeat) {
+            asgn += Boogie.Assign(transExpr(v,acvs), B.Fun("Map#Store",transExpr(v,acvs) , B.Int(i) , B.ChannelIdx(cId, v.typ, B.R(cId)) )  )
+            asgn += Boogie.Assign(B.R(cId), B.R(cId) plus B.Int(1))
+          }
+        }
+      }
+    }
+    
+    for (pre <- action.requires) {
+      if (!pre.free) {
+        asgn += B.Assert(transExprPrecondCheck(pre.expr,acvs),pre.pos,"Precondition might not hold for instance at " + instance.pos)
+      }
+    }
+    
+    asgn ++= generateHavoc(acvs.assignedVariables, acvs)
+    
+    for (opat <- action.outputPattern) {
+      val cId = acvs.connectionMap.getSrc(PortRef(Some(instance.id),opat.portId))
+      if (action.isContractAction) {
+        asgn += Boogie.Assign(B.C(cId),B.C(cId) plus B.Int(opat.rate))
+      }
+      else {
+        val outputPat = opat.asInstanceOf[OutputPattern]
+        if (opat.repeat == 1) {
+          for (e <- outputPat.exps) {
+            asgn += Boogie.Assign(B.ChannelIdx(cId,e.typ,B.C(cId)),transExpr(e,acvs))
+            asgn += Boogie.Assign(B.C(cId),B.C(cId) plus B.Int(1))
+          }
+        }
+        else {
+          val v = outputPat.exps(0)
+          for (i <- 0 until opat.repeat) {
+            asgn += Boogie.Assign(B.ChannelIdx(cId, v.typ, B.C(cId)), B.Fun("Map#Select",transExpr(v,acvs), B.Int(i)))
+            asgn += Boogie.Assign(B.C(cId), B.C(cId) plus B.Int(1))
+          }
+        }
+      }
+    }
+    
+    for (post <- action.ensures) {
+      asgn += B.Assume(transExprPrecondCheck(post.expr,acvs))
+    }
+    
+    for (chi <- acvs.chInvariants) {
+      if (!chi.assertion.free) {
+        val msg = 
+            "Action at " + action.pos + " ('" + action.fullName + "') for actor instance '" + 
+            instance.id + "' might not preserve the channel invariant"
+        asgn += BAssert(chi, msg, acvs)
+      }
+    }
+    
+    asgn.toList
+  }
+  
+  // Contract checking
+  
+  def translateNetworkAction(
+    nwa: ContractAction, nwvs: RootVerStruct[Network], subactorFiringRules: List[Boogie.Expr]): List[Boogie.Decl] = {
+  
     val boogieProcs = new ListBuffer[Boogie.Proc]()
     
     for (ipat <- nwa.inputPattern) {
@@ -165,21 +289,71 @@ class NetworkTranslator(
     boogieProcs.toList
   }
   
+  def translateNetworkInput(action: ContractAction, pattern: NwPattern, nwvs: RootVerStruct[Network]) = {
+    
+    val asgn = new ListBuffer[Boogie.Stmt]()
+    
+    asgn ++= nwvs.declarations.map { _.decl }
+    asgn ++= nwvs.assumes
+    
+//    asgn ++= (nwvs.entityDecls map { _.decl })
+//    asgn ++= nwvs.subactorVarDecls  map { _.decl }
+//    asgn ++= (nwvs.uniquenessConditions map { B.Assume(_) })
+//    asgn ++= nwvs.basicAssumes
+   // asgn += B.Assume(nwvs.actionRatePredicates(action))
+    //asgn += B.Local("x", B.type2BType(IntType(-1)))
+    
+    asgn += B.Assume(B.Mode(B.This) ==@ Boogie.VarExpr(action.fullName))
+    
+    val portType = nwvs.entity.getInport(pattern.portId).get.portType
+    
+    asgn += 
+      B.Assume(
+          (B.C(transExpr(pattern.portId,ChanType(portType),nwvs)) - 
+            B.I(transExpr(pattern.portId,ChanType(portType),nwvs))) < 
+              B.Int(pattern.rate))
+     
+    for (chi <- nwvs.chInvariants) {
+      asgn += BAssume(chi, nwvs)
+    }
+    
+    asgn ++= nwvs.translatedIoInvariants(stmtTranslator) map B.Assume
+    
+    asgn += Boogie.Assign(
+        B.C(transExpr(pattern.portId,ChanType(portType),nwvs)),
+        B.C(transExpr(pattern.portId,ChanType(portType),nwvs)) + B.Int(1))
+    
+    for (g <- action.guards) {
+      asgn += B.Assume(transExpr(g,nwvs))
+    }
+    for (r <- action.requires) {
+      asgn += B.Assume(transExpr(r.expr,nwvs))
+    }
+    
+    
+    for (chi <- nwvs.chInvariants) {
+      if (!chi.assertion.free) {
+        asgn += BAssert(chi, "Channel invariant might be falsified by network input on port '" + pattern.portId + "' for contract '" + action.fullName + "'"  , nwvs)
+      }
+    }
+
+    asgn.toList
+  }
   
-  def transNetworkExit(nwa: ContractAction, nwvs: NetworkVerificationStructure, subactorFiringRules: List[Boogie.Expr]) = {
+  def transNetworkExit(nwa: ContractAction, nwvs: RootVerStruct[Network], subactorFiringRules: List[Boogie.Expr]) = {
     // Network action exit
     
     val inputBounds = 
       nwvs.entity.inports.map { 
         p =>
-          B.Assume(B.C(transExpr(p.id,p.portType)(nwvs.renamings)) - B.I(transExpr(p.id,p.portType)(nwvs.renamings)) ==@ B.Int(nwa.inportRate(p.id)))
+          B.Assume(B.C(transExpr(p.id,p.portType,nwvs)) - B.I(transExpr(p.id,p.portType,nwvs)) ==@ B.Int(nwa.inportRate(p.id)))
       }
     
     val outputBounds = 
       nwvs.entity.outports.map { 
         p =>
           B.Assert(
-              B.C(transExpr(p.id,p.portType)(nwvs.renamings)) - B.I(transExpr(p.id,p.portType)(nwvs.renamings)) ==@ B.Int(nwa.outportRate(p.id)),
+              B.C(transExpr(p.id,p.portType,nwvs)) - B.I(transExpr(p.id,p.portType,nwvs)) ==@ B.Int(nwa.outportRate(p.id)),
               nwa.pos,
               "The correct number of tokens might not be produced on output '" + p.id +  "' for contract '" + nwa.fullName + "'" 
               )
@@ -189,23 +363,26 @@ class NetworkTranslator(
     
     val asgn = new ListBuffer[Boogie.Stmt]
     
-    asgn ++= (nwvs.entityDecls map { _.decl })
-    asgn ++= (nwvs.subactorVarDecls  map { _.decl })
-    asgn ++= (nwvs.uniquenessConditions map {B.Assume(_)})
-    asgn ++= nwvs.basicAssumes
+    asgn ++= nwvs.declarations.map { _.decl }
+    asgn ++= nwvs.assumes
+    
+//    asgn ++= (nwvs.entityDecls map { _.decl })
+//    asgn ++= (nwvs.subactorVarDecls  map { _.decl })
+//    asgn ++= (nwvs.uniquenessConditions map {B.Assume(_)})
+//    asgn ++= nwvs.basicAssumes
     asgn += B.Assume(B.Mode(B.This) ==@ Boogie.VarExpr(nwa.fullName))
-    asgn += B.Assume(nwvs.actionRatePredicates(nwa))
+//    asgn += B.Assume(nwvs.actionRatePredicates(nwa))
     
     for (chi <- nwvs.chInvariants) {
-      asgn += BAssume(chi,nwvs.renamings)
+      asgn += BAssume(chi,nwvs)
     }
-    for ((pinv,renames) <- nwvs.publicSubInvariants) {
-      asgn += BAssume(pinv, renames)
-    }
+    
+    asgn ++= nwvs.translatedIoInvariants(stmtTranslator) map B.Assume
+    
     asgn ++= inputBounds
     
     for (r <- nwa.requires) {
-      asgn += B.Assume(transExpr(r.expr)(nwvs.renamings))
+      asgn += B.Assume(transExpr(r.expr,nwvs))
     }
     
     asgn ++= firingNegAssumes
@@ -213,7 +390,7 @@ class NetworkTranslator(
     
     for (q <- nwa.ensures) {
       if (!q.free) {
-        asgn += B.Assert(transExpr(q.expr)(nwvs.renamings),q.pos,"Network action postcondition might not hold")
+        asgn += B.Assert(transExpr(q.expr,nwvs),q.pos,"Network action postcondition might not hold")
       }
     }
     
@@ -230,172 +407,17 @@ class NetworkTranslator(
     asgn += Boogie.Assign(Boogie.VarExpr(BMap.I), Boogie.VarExpr(BMap.R))
     for (chi <- nwvs.chInvariants) {
       if (!chi.assertion.free) {
-        asgn += BAssert(chi,"The network might not preserve the channel invariant for contract '" + nwa.fullName + "'" ,nwvs.renamings)
+        asgn += BAssert(chi,"The network might not preserve the channel invariant for contract '" + nwa.fullName + "'" ,nwvs)
       }
     }
     
     for (nwi <- nwvs.nwInvariants) {
       if (!nwi.assertion.free) {
-        asgn += BAssert(nwi,"The network might not preserve the network invariant for contract '" + nwa.fullName + "'",nwvs.renamings)
+        asgn += BAssert(nwi,"The network might not preserve the network invariant for contract '" + nwa.fullName + "'",nwvs)
       }
     }
     
     B.createProc(Uniquifier.get(nwvs.namePrefix+nwa.fullName+"#exit"),asgn.toList,smokeTest)
   }
   
-  
-  
-  def transSubActionExecution(
-      instance: Instance, 
-      action: AbstractAction, 
-      nwvs: NetworkVerificationStructure,
-      firingRule: Boogie.Expr): List[Boogie.Stmt] = {
-    
-    val actor = instance.actor
-    val asgn = new ListBuffer[Boogie.Stmt]()
-    
-    asgn ++= nwvs.entityDecls map { _.decl }
-    asgn ++= nwvs.subactorVarDecls  map { _.decl }
-    asgn ++= nwvs.uniquenessConditions map {B.Assume(_)}
-    asgn ++= nwvs.getEntityActionData(instance, action).declarations  map { _.decl }
-    
-    asgn ++= nwvs.basicAssumes
-    
-    for (ip <- instance.actor.inports) {
-      val cId = nwvs.connectionMap.getDst(PortRef(Some(instance.id),ip.id))
-      asgn += Boogie.Assign(B.Isub(cId), B.R(cId))
-    }
-    
-    for (op <- instance.actor.outports) {
-      val cId = nwvs.connectionMap.getSrc(PortRef(Some(instance.id),op.id))
-      asgn += Boogie.Assign(B.Isub(cId), B.C(cId))
-    }
-    
-    asgn ++= (for (chi <- nwvs.chInvariants) yield BAssume(chi,nwvs.renamings))  // Assume channel invariants
-    
-    for ((pinv,renames) <- nwvs.publicSubInvariants) {
-      asgn += BAssume(pinv, renames)
-    }
-    
-    val renamings = nwvs.subActionRenamings(instance, action)
-    
-    val replacementMap = nwvs.getEntityActionData(instance, action).replacements
-    
-    asgn += B.Assume(firingRule)
-    
-    for (ipat <- action.inputPattern) {
-      val cId = nwvs.connectionMap.getDst(PortRef(Some(instance.id),ipat.portId))
-      if (action.isContractAction) {
-        asgn += Boogie.Assign(B.R(cId), B.R(cId) plus B.Int(ipat.rate))
-      }
-      else {
-        val inputPat = ipat.asInstanceOf[InputPattern]
-        if (inputPat.repeat == 1) {
-          for (v <- inputPat.vars) {
-            asgn += Boogie.Assign(transExpr(v.id,v.typ)(renamings),B.ChannelIdx(cId,v.typ,B.R(cId)))
-            asgn += Boogie.Assign(B.R(cId), B.R(cId) plus B.Int(1))
-          }
-        }
-        else {
-          val v = inputPat.vars(0)
-          for (i <- 0 until inputPat.repeat) {
-            asgn += Boogie.Assign(transExpr(v)(renamings), B.Fun("Map#Store",transExpr(v)(renamings) , B.Int(i) , B.ChannelIdx(cId, v.typ, B.R(cId)) )  )
-            asgn += Boogie.Assign(B.R(cId), B.R(cId) plus B.Int(1))
-          }
-        }
-      }
-    }
-    
-    for (pre <- action.requires) {
-      if (!pre.free) {
-        asgn += B.Assert(transExprPrecondCheck(pre.expr)(renamings),pre.pos,"Precondition might not hold for instance at " + instance.pos)
-      }
-    }
-    
-    asgn ++= generateHavoc(nwvs.getEntityActionData(instance, action).assignedVariables, renamings)
-    
-    for (opat <- action.outputPattern) {
-      val cId = nwvs.connectionMap.getSrc(PortRef(Some(instance.id),opat.portId))
-      if (action.isContractAction) {
-        asgn += Boogie.Assign(B.C(cId),B.C(cId) plus B.Int(opat.rate))
-      }
-      else {
-        val outputPat = opat.asInstanceOf[OutputPattern]
-        if (opat.repeat == 1) {
-          for (e <- outputPat.exps) {
-            asgn += Boogie.Assign(B.ChannelIdx(cId,e.typ,B.C(cId)),transExpr(e)(renamings))
-            asgn += Boogie.Assign(B.C(cId),B.C(cId) plus B.Int(1))
-          }
-        }
-        else {
-          val v = outputPat.exps(0)
-          for (i <- 0 until opat.repeat) {
-            asgn += Boogie.Assign(B.ChannelIdx(cId, v.typ, B.C(cId)), B.Fun("Map#Select",transExpr(v)(renamings), B.Int(i)))
-            asgn += Boogie.Assign(B.C(cId), B.C(cId) plus B.Int(1))
-          }
-        }
-      }
-    }
-    
-    for (post <- action.ensures) {
-      asgn += B.Assume(transExprPrecondCheck(post.expr)(renamings))
-    }
-    
-    for (chi <- nwvs.chInvariants) {
-      if (!chi.assertion.free) {
-        val msg = 
-            "Action at " + action.pos + " ('" + action.fullName + "') for actor instance '" + 
-            instance.id + "' might not preserve the channel invariant"
-        asgn += BAssert(chi, msg, nwvs.renamings)
-      }
-    }
-    
-    asgn.toList
-  }
-  
-  
-  
-  def translateNetworkInput(action: ContractAction, pattern: NwPattern, nwvs: NetworkVerificationStructure) = {
-    
-    val asgn = new ListBuffer[Boogie.Stmt]()
-    asgn ++= (nwvs.entityDecls map { _.decl })
-    asgn ++= nwvs.subactorVarDecls  map { _.decl }
-    asgn ++= (nwvs.uniquenessConditions map { B.Assume(_) })
-    asgn ++= nwvs.basicAssumes
-    asgn += B.Assume(nwvs.actionRatePredicates(action))
-    //asgn += B.Local("x", B.type2BType(IntType(-1)))
-    asgn += B.Assume(B.Mode(B.This) ==@ Boogie.VarExpr(action.fullName))
-    
-    val portType = nwvs.entity.getInport(pattern.portId).get.portType
-    
-    asgn += 
-      B.Assume(B.C(transExpr(pattern.portId,ChanType(portType))(nwvs.renamings)) - B.I(transExpr(pattern.portId,ChanType(portType))(nwvs.renamings)) < B.Int(pattern.rate))
-     
-    for (chi <- nwvs.chInvariants) {
-      asgn += BAssume(chi, nwvs.renamings)
-    }
-    
-    for ((pinv,renames) <- nwvs.publicSubInvariants) {
-      asgn += BAssume(pinv, renames)
-    }
-    asgn += Boogie.Assign(
-        B.C(transExpr(pattern.portId,ChanType(portType))(nwvs.renamings)),
-        B.C(transExpr(pattern.portId,ChanType(portType))(nwvs.renamings)) + B.Int(1))
-    
-    for (g <- action.guards) {
-      asgn += B.Assume(transExpr(g)(nwvs.renamings))
-    }
-    for (r <- action.requires) {
-      asgn += B.Assume(transExpr(r.expr)(nwvs.renamings))
-    }
-    
-    
-    for (chi <- nwvs.chInvariants) {
-      if (!chi.assertion.free) {
-        asgn += BAssert(chi, "Channel invariant might be falsified by network input on port '" + pattern.portId + "' for contract '" + action.fullName + "'"  , nwvs.renamings)
-      }
-    }
-
-    asgn.toList
-  }
 }
