src/main/scala/fi/abo/it/actortool/boogie/VerStruct.scala
@@ -1,6 +1,8 @@
 package fi.abo.it.actortool.boogie
 
 import fi.abo.it.actortool._
+import fi.abo.it.actortool.schedule._
+import fi.abo.it.actortool.util.ConnectionMap
 import fi.abo.it.actortool.util.PriorityMapBuilder
 import collection.mutable.ListBuffer
 
@@ -8,13 +10,22 @@ trait VerStruct[T] {
   def entity: T
   def namePrefix: String
   def renamings: Map[String,Expr] = Map.empty
-  def declarations: List[BDecl] = List.empty
-  def assumes = List.empty[Boogie.Assume]
+  def declarations: Seq[BDecl] = Seq.empty
+  def assumes = Seq.empty[Boogie.Assume]
+  def stateChannelNames: Map[String,Id] = Map.empty
+  def entities: Seq[Instance] = Seq.empty
+  def connections: Seq[Connection] = Seq.empty
+  def nwInvariants: Seq[ActorInvariant] = Seq.empty
+  def chInvariants: Seq[ChannelInvariant] = Seq.empty
+  def connectionMap: ConnectionMap = ConnectionMap.empty
+  def translatedIoInvariants(t: StmtExpTranslator): Seq[Boogie.Expr] = Seq.empty
 }
+
 
 trait RootVerStruct[T<:DFActor] extends VerStruct[T] {
   def contracts: Seq[ContractAction]
-  def priorities(useContracts: Boolean) = PriorityMapBuilder.buildPriorityMap(entity, false, useContracts)
+  def priorities(useContracts: Boolean) = 
+    PriorityMapBuilder.buildPriorityMap(entity, false, useContracts)
 }
 
 trait ChildVerStruct[T,P] extends VerStruct[T] {
@@ -22,6 +33,16 @@ trait ChildVerStruct[T,P] extends VerStruct[T] {
   override def renamings = parent.renamings
   override def declarations = parent.declarations
   override def assumes = parent.assumes
+  override def stateChannelNames = parent.stateChannelNames
+  override def connections: Seq[Connection] = parent.connections
+  override def nwInvariants: Seq[ActorInvariant] = parent.nwInvariants
+  override def chInvariants: Seq[ChannelInvariant] = parent.chInvariants
+  override def connectionMap: ConnectionMap = parent.connectionMap
+  override def translatedIoInvariants(t: StmtExpTranslator): Seq[Boogie.Expr] = parent.translatedIoInvariants(t)
+}
+
+trait ActionExecVerStruct[T,P] extends ChildVerStruct[T,P] {
+  def assignedVariables: Set[Assignable]
 }
 
 class ActorVerStruct(
@@ -29,7 +50,7 @@ class ActorVerStruct(
     override val declarations: List[BDecl],
     override val assumes: List[Boogie.Assume],
     val functionNames: Map[String,Id],
-    val stateChannelNames: Map[String,Id]
+    override val stateChannelNames: Map[String,Id]
     ) extends RootVerStruct[BasicActor] {
   
   override def contracts = entity.contractActions
@@ -42,44 +63,82 @@ class NetworkVerStruct(
     override val entity: Network,
     override val declarations: List[BDecl],
     override val assumes: List[Boogie.Assume],
-    val stateChannelNames: Map[String,Id],
-    override val renamings: Map[String,Id]
+    override val stateChannelNames: Map[String,Id],
+    override val renamings: Map[String,Id],
+    val ioInvariants: List[(Instance,List[Invariant])]
     ) extends RootVerStruct[Network] {
   
   override def contracts = entity.contractActions
   override def namePrefix = entity.id
+  override def connectionMap = ConnectionMap.build(entity.structure.get.connections, renamings)
+  
+  override def entities = entity.entities.get.entities
+  override def connections = entity.structure.get.connections
+  override def nwInvariants = entity.actorInvariants
+  override def chInvariants = entity.channelInvariants
+  
+  override def translatedIoInvariants(translator: StmtExpTranslator) = {
+    (for ((e,invs) <- ioInvariants) yield {
+      val ivs = VerStruct(this, e)
+      val ctx = TranslatorContext(ivs.renamings,false)
+      for (i <- invs) yield {
+        translator.transExpr(i.expr,ctx)
+      }
+    }) flatten
+  }
   
 }
 
 class ActionVerStruct(
-    override val parent: ActorVerStruct,
+    override val parent: RootVerStruct[BasicActor],
     override val entity: ActorAction,
     val actionDeclarations: List[BDecl],
-    val actionAssumes: List[Boogie.Assume]
-    ) extends ChildVerStruct[ActorAction,BasicActor] {
+    val actionAssumes: List[Boogie.Assume],
+    val actionVariableInits: List[Expr],
+    val guard: GuardTranslation
+    ) extends ActionExecVerStruct[ActorAction,BasicActor] {
   
   override def namePrefix = parent.namePrefix + B.Sep + entity.fullName
-  override def declarations = parent.declarations ::: actionDeclarations
-  override def assumes = parent.assumes ::: actionAssumes
-  def assignedVariables = AssignedVarsFinder.find(entity.body)
+  override def declarations = parent.declarations ++ actionDeclarations
+  override def assumes = parent.assumes ++ actionAssumes
+  override def assignedVariables = AssignedVarsFinder.find(entity.body)
+  override def renamings = parent.renamings ++ guard.renamings
   
 }
 
 class InstanceVerStruct(
-    override val parent: NetworkVerStruct,
-    override val entity: Instance
-    ) extends ChildVerStruct[Instance,Network] {
+    override val parent: RootVerStruct[Network],
+    override val entity: Instance,
+    val paramRenamings: Map[String,Expr]) extends ChildVerStruct[Instance,Network] {
   
   override def namePrefix = parent.namePrefix + B.Sep + entity.id
+  
+  def priorities(useContracts: Boolean) = 
+    PriorityMapBuilder.buildPriorityMap(entity.actor, true, useContracts)
+  
+  override def renamings = parent.renamings ++ paramRenamings
   
 }
 
 class SubActionVerStruct(
     override val parent: InstanceVerStruct,
-    override val entity: AbstractAction
-    ) extends ChildVerStruct[AbstractAction,Instance] {
+    override val entity: AbstractAction,
+    val actionDecls: List[BDecl],
+    val replacements: Map[Id,Expr],
+    val subactionRenamings: Map[String,Id]
+    ) extends ActionExecVerStruct[AbstractAction,Instance] {
   
   override def namePrefix = parent.namePrefix + B.Sep + entity.fullName
+  override def connectionMap = parent.connectionMap
+  
+  def priorities(useContracts: Boolean) = {
+    parent.priorities(useContracts)
+  }
+  
+  override def assignedVariables = AssignedVarsFinder.find(entity.body)
+  
+  override def renamings = parent.renamings ++ subactionRenamings
+  override def declarations = parent.declarations ++ actionDecls
   
 }
 
@@ -90,11 +149,15 @@ object VerStruct {
     val decls = new ListBuffer[BDecl]
     val assumes = new ListBuffer[Boogie.Assume]
     val stateChannelNames = collection.mutable.Map[String,Id]()
-    val actionVerStructs = new ListBuffer[ActionVerStruct]
+    
     
     // Declaration of ports
     for (p <- actor.inports ::: actor.outports) {
       decls += BDecl(p.id, ChanType(p.portType)) 
+    }
+    
+    for (p <- actor.parameters) {
+      decls += BDecl(p.id,p.typ)
     }
     
     // Declaration of virtual channels for actor variables
@@ -110,8 +173,8 @@ object VerStruct {
         p => B.Assume(B.Int(0) <= B.I(p.id) && B.I(p.id) <= B.R(p.id) && B.R(p.id) <= B.C(p.id)) 
       }
     assumes ++=
-      stateChannelNames.keys map { 
-        k => B.Assume(B.Int(0) <= B.I(k) && B.I(k) <= B.R(k) && B.R(k) <= B.C(k)) 
+      stateChannelNames.values map { 
+        k => B.Assume(B.Int(0) <= B.I(k.id) && B.I(k.id) <= B.R(k.id) && B.R(k.id) <= B.C(k.id)) 
       }
     
     val (contractModeDecls, contractModeAssumes) = createContractModeDeclsAndAssumes(actor)
@@ -123,8 +186,8 @@ object VerStruct {
     decls ++= variableDecls
     assumes ++= variableAssumes
     
-    val priorityMap = PriorityMapBuilder.buildPriorityMap(actor, false, useContracts)
-    val funDeclRenamings = actor.functionDecls.map(fd =>  fd.name -> Id(actor.fullName+B.Sep+fd.name))
+    val funDeclRenamings = 
+      actor.functionDecls.map(fd =>  fd.name -> Id(actor.fullName+B.Sep+fd.name))
     
     new ActorVerStruct(
         actor,
@@ -135,40 +198,10 @@ object VerStruct {
         )
   }
   
-  def apply(parent: ActorVerStruct, action: ActorAction, useContracts: Boolean) = {
+  
+  def apply(network: Network, useContracts: Boolean): RootVerStruct[Network] = {
     
     val stmtTranslator = new StmtExpTranslator
-    val transCtx = TranslatorContext(parent.renamings, false, parent.stateChannelNames)
-    
-    val decls = new ListBuffer[BDecl]
-    val assumes = new ListBuffer[Boogie.Assume]
-    
-    if (action.init) {
-      assumes ++= 
-        parent.entity.inports:::parent.entity.outports map { 
-          p => B.Assume(B.I(p.id) ==@ B.Int(0) && B.R(p.id) ==@ B.Int(0) && B.C(p.id) ==@ B.Int(0)) 
-        }
-      assumes ++= 
-        parent.stateChannelNames.keys map { 
-          k => B.Assume(B.I(k) ==@ B.Int(0) && B.R(k) ==@ B.Int(0) && B.C(k) ==@ B.Int(0)) 
-        }
-    }
-    else {
-      assumes ++= parent.stateChannelNames.keys.map { k => B.Assume((B.R(k) + B.Int(1)) ==@ B.C(k)) }
-    }
-    
-    for (d <- action.variables) {
-      decls += BDecl(d.id,d.typ)
-      if (d.constant) {
-        assumes += Boogie.Assume(Boogie.VarExpr(d.id) ==@  stmtTranslator.transExpr(d.value.get, transCtx))
-      }
-    }
-    
-    new ActionVerStruct(parent,action,decls.toList,assumes.toList)
-  }
-  
-  
-  def apply(network: Network, useContracts: Boolean) = {
     
     val decls = new ListBuffer[BDecl]
     val assumes = new ListBuffer[Boogie.Assume]
@@ -182,18 +215,47 @@ object VerStruct {
     decls ++= contractModeDecls
     assumes ++= contractModeAssumes
     
+    val channels = new ListBuffer[BDecl]
+    
+    for (c <- connections) {
+      renamings += c.id -> Id(namePrefix+B.Sep+c.id).withType(c.typ)
+      channels += BDecl(namePrefix+B.Sep+c.id,c.typ)
+    }
+    
+    //val transCtx = TranslatorContext(renamings.toMap, false, Map.empty)
+    
+    val ioInvariants = new ListBuffer[(Instance,List[Invariant])]
+    for (e <- entities) {
+      ioInvariants += e -> e.actor.streamInvariants
+    }
+    
+    decls ++= channels
+    assumes += B.Assume(createUniquenessCondition(channels.toList))
+    
+    val tempRenamings = renamings.toMap
+    
+    for (c <- connections) {
+      val tempRenamings = renamings.toMap
+      val name = tempRenamings(c.id)
+      assumes += 
+        B.Assume(B.Int(0) <= B.I(name.id) && B.I(name.id) <= B.R(name.id) && B.R(name.id) <= B.C(name.id))      
+      if (c.isOutput) {
+        assumes += B.Assume(B.I(name.id) ==@ B.R(name.id))
+      }
+    }
+    
     // Add input/output port names as synonyms to the connected channels
     for (ip <- network.inports) {
       val ch = network.structure.get.getInputChannel(ip.id)
       ch match {
-        case Some(c) => renamings += ip.id -> Id(namePrefix+c.id).withType(c.typ)
+        case Some(c) => renamings += ip.id -> Id(namePrefix+B.Sep+c.id).withType(c.typ)
         case None =>
       }
     }
     for (op <- network.outports) {
       val ch = network.structure.get.getOutputChannel(op.id)
       ch match {
-        case Some(c) => renamings += op.id -> Id(namePrefix+c.id).withType(c.typ)
+        case Some(c) => renamings += op.id -> Id(namePrefix+B.Sep+c.id).withType(c.typ)
         case None =>
       }
     }
@@ -203,17 +265,134 @@ object VerStruct {
         decls.toList,
         assumes.toList,
         Map.empty, // State channels
-        renamings.toMap
+        renamings.toMap,
+        ioInvariants.toList
         )
           
   }
   
-  def apply(parent: NetworkVerStruct, instance: Instance) = {
-    new InstanceVerStruct(parent,instance)
+  def apply(parent: RootVerStruct[BasicActor], action: ActorAction, guard: GuardTranslation): ActionVerStruct = 
+    apply(parent,action,guard,false)
+  
+  def apply(
+      parent: RootVerStruct[BasicActor], 
+      action: ActorAction, 
+      guard: GuardTranslation,
+      includePatternVars: Boolean): ActionVerStruct = {
+    
+    val stmtTranslator = new StmtExpTranslator
+    val transCtx = TranslatorContext(parent.renamings, false, parent.stateChannelNames)
+    
+    val decls = new ListBuffer[BDecl]
+    val assumes = new ListBuffer[Boogie.Assume]
+    val actionVariableInits = new ListBuffer[Expr]
+    
+    if (action.init) {
+      assumes ++= 
+        (parent.entity.inports ++ parent.entity.outports) map { 
+          p => B.Assume(B.I(p.id) ==@ B.Int(0) && B.R(p.id) ==@ B.Int(0) && B.C(p.id) ==@ B.Int(0)) 
+        }
+      assumes ++= 
+        parent.stateChannelNames.values map { 
+          k => B.Assume(B.I(k.id) ==@ B.Int(0) && B.R(k.id) ==@ B.Int(0) && B.C(k.id) ==@ B.Int(0)) 
+        }
+    }
+    else {
+      assumes ++= parent.stateChannelNames.values.map { k => B.Assume((B.R(k.id) + B.Int(1)) ==@ B.C(k.id)) }
+    }
+    
+    for (d <- action.variables) {
+      decls += BDecl(d.id,d.typ)
+      if (d.constant) {
+        val id = Id(d.id).withType(d.typ)
+        val exp = Eq(id, d.value.get).withType(BoolType)
+        
+        actionVariableInits += exp
+      }
+    }
+    
+    decls ++= guard.declarations
+    
+    new ActionVerStruct(parent,action,decls.toList,assumes.toList,actionVariableInits.toList,guard)
+  }
+  
+  
+  
+  
+  def apply(parent: RootVerStruct[Network], instance: Instance) = {
+    
+    val renamings = new ListBuffer[(String,Expr)]
+    
+    renamings ++= instance.actor.parameters.map(_.id).zip(instance.arguments)
+    
+    for (p <- instance.actor.inports) {
+      val newName = parent.connectionMap.getDst(instance.id,p.id)
+      renamings += p.id -> Id(newName).withType(ChanType(p.portType))
+    }
+    
+    for (p <- instance.actor.outports) {
+      val newName = parent.connectionMap.getSrc(instance.id,p.id)
+      renamings += p.id -> Id(newName).withType(ChanType(p.portType))
+    }
+    
+//    for (v <- instance.actor.variables) {
+//      println(instance.actor.fullName, v.id)
+//    }
+    
+    new InstanceVerStruct(parent, instance, renamings.toMap)
   }
   
   def apply(parent: InstanceVerStruct, action: AbstractAction) = {
-    new SubActionVerStruct(parent,action)
+    
+    val instance = parent.entity
+    
+    val actor = instance.actor
+    val vars = new ListBuffer[BDecl]()
+    
+    val replacements = scala.collection.mutable.HashMap.empty[Id,Expr]
+    
+    action match {
+      case ac: ActorAction => {
+        for (ipat <- ac.inputPattern) {
+          val cId = parent.connectionMap.getDst(instance.id,ipat.portId)      
+          for ((v,ind) <- ipat.vars.zipWithIndex) {
+            val c = Elements.ch(cId,v.typ)
+            val index = 
+              if (ind == 0) Elements.rd(c.id,c.typ.asInstanceOf[ChanType]) 
+              else Minus(Elements.rd(c.id,c.typ.asInstanceOf[ChanType]),IntLiteral(ind))
+            val acc = Elements.chAcc(c,index)
+            replacements += (v -> acc)
+          }
+        }
+        
+        val patternVarRenamings: Map[String,Id] = {
+          if (instance.actor.isNetwork) Map.empty
+          else {
+            ((for (ipat <- ac.inputPattern) yield {
+              for (v <- ipat.vars) yield {
+                val inVar = instance.id + B.Sep + ipat.portId + B.Sep + v.id
+                vars += BDecl(inVar,B.Local(inVar,B.type2BType(v.typ)))
+                (v.id, Id(inVar).withType(v.typ))
+              }
+            }).flatten :::
+            (action.variables.map { 
+              v => {
+                val actionVar = instance.id + B.Sep + action.fullName + B.Sep + v.id
+                vars += BDecl(actionVar,B.Local(actionVar,B.type2BType(v.typ)))
+                (v.id,Id(actionVar).withType(v.typ))
+              }
+            })
+            ).toMap
+          }
+        }
+        
+        new SubActionVerStruct(parent, action, vars.toList, replacements.toMap, patternVarRenamings.toMap)
+      }
+      case c: ContractAction => {
+        new SubActionVerStruct(parent, action, List.empty, Map.empty, Map.empty)
+      }
+    }
+    
   }
   
   protected def createUniquenessCondition(names: List[BDecl]): Boogie.Expr = {
